theories/prob_eff_lang/probblaze/typing/fundamental.v
@@ -3,6 +3,7 @@ From iris.proofmode Require Import proofmode.
 From clutch.prelude Require Import stdpp_ext. 
 From clutch.prob_eff_lang.probblaze Require Import metatheory notation syntax semantics sem_judgement sem_def.
 From clutch.prob_eff_lang.probblaze Require Import primitive_laws compatibility.
+From clutch.prob_eff_lang.probblaze Require Import sem_env.
 From clutch.prob_eff_lang.probblaze Require Import types.
 From clutch.prob_eff_lang.probblaze Require Import interp logic.
 
@@ -11,10 +12,22 @@ Section fundamental.
 
 Lemma ctx_dom_env_dom x Γ :
   ∀ η μ δ ξ, x ∉ ctx_dom Γ → x ∉ env_dom ((λ '(s, τ), (s, interp._ty η μ δ τ ξ)) <$> Γ).
-Proof. 
-  iIntros (???? Hnin).
-  induction Γ as [| (y, κ) Γ' IH]; first set_solver; simpl.
-Admitted. 
+Proof.
+  intros η μ δ ξ Hnin. induction Γ as [| (y, κ) Γ' IH]; simpl.
+  - rewrite env_dom_nil. apply not_elem_of_nil.
+  - rewrite env_dom_cons. apply not_elem_of_cons. split.
+    + intros ->. apply Hnin. rewrite /ctx_dom /=. set_solver.
+    + apply IH. rewrite /ctx_dom /= in Hnin. set_solver.
+Qed.
+
+(* Extract the bare relational interpretation of a value from its semantic
+   value-typing judgement, at a given interpretation environment. *)
+Lemma sem_val_related_interp (v : val) (τ : type) η μ δ ξ :
+  (⊢ ⊨ᵥ v ≤log≤ v : τ) → ⊢ interp._ty η μ δ τ ξ v v.
+Proof.
+  iIntros (H). iPoseProof H as "H". iDestruct ("H" $! η μ δ ξ) as "H'".
+  iEval (rewrite /sem_val_typed /tc_opaque) in "H'". iApply "H'".
+Qed.
 
 Theorem fundamental Δ Γ1 e ρ τ Γ2 :
   Δ .| Γ1 ⊢ₜ e : ρ : τ ⊣ Γ2 → ⊢ 〈Δ;Γ1〉 ⊨ₜ e ≤log≤ e : ρ : τ ⫤ Γ2
@@ -23,48 +36,108 @@ Theorem fundamental Δ Γ1 e ρ τ Γ2 :
   with fundamental_pure Γ e τ :
     Γ ⊢ₚ e : τ → ⊢ bin_log_pure_related Γ e e τ.
 Proof.
-  - intros Ht. destruct Ht; iIntros (??????).
-    + iApply sem_typed_var.
-    + iApply sem_typed_val; by iApply fundamental_val.
-    + rewrite fmap_app. iApply sem_typed_oval.
+  - intros Ht. destruct Ht; iIntros (η μ δ ξ vs Hδ).
+    + (* Var_typed *) iApply sem_typed_var.
+    + (* Val_typed *) iApply sem_typed_val; by iApply fundamental_val.
+    + (* Pure_typed *) rewrite fmap_app. iApply sem_typed_oval.
       by iApply fundamental_pure.
-    + iApply sem_typed_pair_gen ;
+    + (* Pair_typed *) iApply sem_typed_pair_gen ;
         (* waiting for syntactic rule for sem_row.RowTypeSub *)
         [admit|apply fundamental in Ht1 as Ht|apply fundamental in Ht2 as Ht];
-        iPoseProof Ht as "Ht"; iSpecialize ("Ht" $! _ _ _ _ _ _); iApply "Ht".
-    + iApply sem_typed_fst_expr. apply fundamental in Ht. 
-        iPoseProof Ht as "Ht"; iSpecialize ("Ht" $! _ _ _ _ _ _); iApply "Ht".
-    + iApply sem_typed_snd_expr. apply fundamental in Ht. 
-        iPoseProof Ht as "Ht"; iSpecialize ("Ht" $! _ _ _ _ _ _); iApply "Ht".
-    + iApply sem_typed_left_inj.
-      apply fundamental in Ht. 
-      iPoseProof Ht as "Ht"; iSpecialize ("Ht" $! _ _ _ _ _ _); iApply "Ht".
-    + iApply sem_typed_right_inj.
-      apply fundamental in Ht. 
-      iPoseProof Ht as "Ht"; iSpecialize ("Ht" $! _ _ _ _ _ _); iApply "Ht".
-    + iApply sem_typed_match.
-      * destruct x; [|eapply ctx_dom_env_dom]; apply H. 
-      * destruct x; [|eapply ctx_dom_env_dom]; apply H0. 
-      * destruct y; [|eapply ctx_dom_env_dom]; apply H1. 
-      * destruct y; [|eapply ctx_dom_env_dom]; apply H2. 
-      * apply fundamental in Ht1. 
-        iPoseProof Ht1 as "Ht"; iSpecialize ("Ht" $! _ _ _ _ _ _); iApply "Ht". 
-      * apply fundamental in Ht2. 
-        iPoseProof Ht2 as "Ht"; iSpecialize ("Ht" $! _ _ _ _ _ _). destruct x; iApply "Ht". 
-      * apply fundamental in Ht3. 
-        iPoseProof Ht3 as "Ht"; iSpecialize ("Ht" $! _ _ _ _ _ _). destruct y; iApply "Ht". 
-    + iApply sem_typed_if.
-      * apply fundamental in Ht1.
-        iPoseProof Ht1 as "Ht"; iSpecialize ("Ht" $! _ _ _ _ _ _); iApply "Ht".
-      * apply fundamental in Ht2.
-        iPoseProof Ht2 as "Ht"; iSpecialize ("Ht" $! _ _ _ _ _ _). iApply "Ht".
-      * apply fundamental in Ht3.
-        iPoseProof Ht3 as "Ht"; iSpecialize ("Ht" $! _ _ _ _ _ _). iApply "Ht".
-    + rewrite fmap_app.
-(*       iApply sem_typed_oval.
-         iApply sem_oval_typed_ufun.
-   1 1 *)
-
-Admitted. 
+        iPoseProof Ht as "Ht"; iApply ("Ht" $! _ _ _ _ ∅ Hδ).
+    + (* Fst_typed *) iApply sem_typed_fst_expr. apply fundamental in Ht.
+      iPoseProof Ht as "Ht". iApply ("Ht" $! _ _ _ _ ∅ Hδ).
+    + (* Snd_typed *) iApply sem_typed_snd_expr. apply fundamental in Ht.
+      iPoseProof Ht as "Ht". iApply ("Ht" $! _ _ _ _ ∅ Hδ).
+    + (* InjL_typed *) iApply sem_typed_left_inj. apply fundamental in Ht.
+      iPoseProof Ht as "Ht". iApply ("Ht" $! _ _ _ _ ∅ Hδ).
+    + (* InjR_typed *) iApply sem_typed_right_inj. apply fundamental in Ht.
+      iPoseProof Ht as "Ht". iApply ("Ht" $! _ _ _ _ ∅ Hδ).
+    + (* Match_typed *) iApply sem_typed_match;
+        [ destruct x; [|eapply ctx_dom_env_dom]; apply H
+        | destruct x; [|eapply ctx_dom_env_dom]; apply H0
+        | destruct y; [|eapply ctx_dom_env_dom]; apply H1
+        | destruct y; [|eapply ctx_dom_env_dom]; apply H2
+        | apply fundamental in Ht1; iPoseProof Ht1 as "Ht";
+            iApply ("Ht" $! _ _ _ _ ∅ Hδ)
+        | apply fundamental in Ht2; iPoseProof Ht2 as "Ht";
+            destruct x; iApply ("Ht" $! _ _ _ _ ∅ Hδ)
+        | apply fundamental in Ht3; iPoseProof Ht3 as "Ht";
+            destruct y; iApply ("Ht" $! _ _ _ _ ∅ Hδ) ].
+    + (* If_typed *) iApply sem_typed_if;
+        [ apply fundamental in Ht1; iPoseProof Ht1 as "Ht";
+            iApply ("Ht" $! _ _ _ _ ∅ Hδ)
+        | apply fundamental in Ht2; iPoseProof Ht2 as "Ht";
+            iApply ("Ht" $! _ _ _ _ ∅ Hδ)
+        | apply fundamental in Ht3; iPoseProof Ht3 as "Ht";
+            iApply ("Ht" $! _ _ _ _ ∅ Hδ) ].
+    + (* Rec_typed *) admit.
+    + (* App_typed *) admit.
+    + (* TAbsElim_typed *) admit.
+    + (* RAbsElim_typed *) admit.
+    + (* MAbsElim_typed *) admit.
+    + (* TAlloc *) iApply sem_typed_alloc. apply fundamental in Ht.
+      iPoseProof Ht as "Ht". iApply ("Ht" $! _ _ _ _ ∅ Hδ).
+    + (* TLoad *) admit.
+    + (* TStore *) admit.
+    + (* TAllocTape *) admit.
+    + (* TRand *) admit.
+    + (* TRandU *) admit.
+    + (* TFold *) admit.
+    + (* TUnfold *) admit.
+    + (* TPack *) admit.
+    + (* TUnpack *) admit.
+    + (* Effect_typed *) admit.
+    + (* Do_typed *) admit.
+    + (* DeepHandle_typed *) admit.
+    + (* ShallowHandle_typed *) admit.
+    + (* Sub_typed *) admit.
+    + (* Contraction_typed *) admit.
+    + (* Weakening_typed *) destruct x; simpl.
+      * apply fundamental in Ht. iPoseProof Ht as "Ht".
+        iApply ("Ht" $! _ _ _ _ ∅ Hδ).
+      * iApply sem_typed_weaken. apply fundamental in Ht.
+        iPoseProof Ht as "Ht". iApply ("Ht" $! _ _ _ _ ∅ Hδ).
+  - intros Hv. destruct Hv; iIntros (η μ δ ξ).
+    + (* Unit_val_typed *) rewrite /sem_val_typed /=. iModIntro. done.
+    + (* Int_val_typed *) rewrite /sem_val_typed /=. iModIntro. eauto.
+    + (* Nat_val_typed *) rewrite /sem_val_typed /=. iModIntro. eauto.
+    + (* Bool_val_typed *) rewrite /sem_val_typed /=. iModIntro. eauto.
+    + (* Pair_val_typed *) apply fundamental_val in Hv1, Hv2.
+      rewrite /sem_val_typed /=. iModIntro.
+      iExists v1, v1, v2, v2. iSplit; first done. iSplit; first done.
+      iSplitL; [iApply (sem_val_related_interp _ _ _ _ _ _ Hv1)
+               |iApply (sem_val_related_interp _ _ _ _ _ _ Hv2)].
+    + (* InjL_val_typed *) apply fundamental_val in Hv.
+      rewrite /sem_val_typed /=. iModIntro. iExists v, v. iLeft.
+      iSplit; first done. iSplit; first done.
+      iApply (sem_val_related_interp _ _ _ _ _ _ Hv).
+    + (* InjR_val_typed *) apply fundamental_val in Hv.
+      rewrite /sem_val_typed /=. iModIntro. iExists v, v. iRight.
+      iSplit; first done. iSplit; first done.
+      iApply (sem_val_related_interp _ _ _ _ _ _ Hv).
+    + (* Rec_val_typed *) admit.
+    + (* TAbs_val_typed *) apply fundamental_val in Hv.
+      rewrite /sem_val_typed /=. iModIntro. iIntros (τ0).
+      iApply (sem_val_related_interp v τ (τ0 :: η) μ δ ξ Hv).
+    + (* RAbs_val_typed *) apply fundamental_val in Hv.
+      rewrite /sem_val_typed /=. iModIntro. iIntros (θ).
+      iApply (sem_val_related_interp v τ η μ δ (θ :: ξ) Hv).
+    + (* MAbs_val_typed *) apply fundamental_val in Hv.
+      rewrite /sem_val_typed /=. iModIntro. iIntros (m).
+      iApply (sem_val_related_interp v τ η (m :: μ) δ ξ Hv).
+  - intros Hp. destruct Hp; iIntros (η μ δ ξ).
+    + (* Val_pure_typed *) apply fundamental_val in H. iPoseProof H as "H".
+      iSpecialize ("H" $! η μ δ ξ). iApply sem_oval_typed_val. iApply "H".
+    + (* Rec_pure_typed *) admit.
+    + (* Pair_pure_typed *) admit.
+    + (* InjL_pure_typed *) admit.
+    + (* InjR_pure_typed *) admit.
+    + (* Var_pure_typed *) admit.
+    + (* BangIntro_pure_typed *) admit.
+    + (* TAbs_pure_typed *) admit.
+    + (* RAbs_pure_typed *) admit.
+    + (* MAbs_pure_typed *) admit.
+Admitted.
 
 End fundamental.
